code/experimental/rsa/Hacl.Impl.Multiplication.fst
@@ -7,6 +7,8 @@ open Spec.Lib.IntTypes
 open FStar.Mul
 
 open Hacl.Impl.Lib
+open Hacl.Impl.Comparison
+open Hacl.Impl.Addition
 
 module Buffer = Spec.Lib.IntBuf
 
@@ -81,3 +83,137 @@ val bn_mul:
         
 let bn_mul #aLen #bLen caLen a cbLen b res = 
     bn_mul_ #aLen #bLen #(aLen + bLen) caLen a cbLen b cbLen (add #SIZE caLen cbLen) res
+
+
+val abs:
+    #aLen:size_nat ->
+    aaLen:size_t{v aaLen == aLen} ->
+    a:lbignum aLen -> b:lbignum aLen -> 
+    res:lbignum aLen -> Stack unit
+    (requires (fun h -> live h a /\ live h b /\ live h res /\ disjoint a b))
+    (ensures  (fun h0 _ h1 -> preserves_live h0 h1 /\ modifies1 res h0 h1))
+
+let abs #aLen aaLen a b res =
+    if (bn_is_less aaLen a b) then
+       //a < b ==> res = b - a
+       bn_sub aaLen b aaLen a res
+    else bn_sub aaLen a aaLen b res
+
+type sign =
+     | Positive : sign
+     | Negative : sign
+
+val add_sign:
+    #aLen:size_nat -> #cLen:size_nat -> #resLen:size_nat ->
+    aaLen:size_t{v aaLen == aLen} ->
+    ccLen:size_t{v ccLen == cLen /\ cLen = aLen + aLen} ->
+    rresLen:size_t{v rresLen == resLen /\ resLen = cLen + 1} ->
+    c0:lbignum cLen -> c1:lbignum cLen -> c2:lbignum cLen ->
+    a0:lbignum aLen -> a1:lbignum aLen -> a2:lbignum aLen ->
+    b0:lbignum aLen -> b1:lbignum aLen -> b2:lbignum aLen ->
+    res:lbignum cLen -> Stack unit
+    (requires (fun h -> live h c0 /\ live h c1 /\ live h c2 /\ 
+                      live h a0 /\ live h a1 /\ live h a2 /\
+                      live h b0 /\ live h b1 /\ live h b2 /\
+		      live h res /\ disjoint a0 a1 /\ disjoint b0 b1))
+    (ensures (fun h0 _ h1 -> preserves_live h0 h1 /\ modifies1 res h0 h1))
+
+let add_sign #aLen #cLen #resLen aaLen ccLen rresLen c0 c1 c2 a0 a1 a2 b0 b1 b2 res =
+    let sa2 = if (bn_is_less aaLen a0 a1) then Negative else Positive in
+    let sb2 = if (bn_is_less aaLen b0 b1) then Negative else Positive in
+    bn_add_carry ccLen c0 ccLen c1 res;
+    if ((sa2 = Positive && sb2 = Positive) || (sa2 = Negative && sb2 = Negative))
+    then bn_sub rresLen res ccLen c2 res
+    else bn_add rresLen res ccLen c2 res
+    
+// iLen is the upper bound for a and b
+// iLen must be a power of 2
+val karatsuba_:
+    #aLen:size_nat ->
+    aaLen:size_t{v aaLen == aLen /\ 4 * aLen < max_size_t} ->
+    a:lbignum aLen -> b:lbignum aLen ->
+    tmp:lbignum (4 * aLen) ->
+    res:lbignum (aLen + aLen) -> Stack unit
+    (requires (fun h -> live h a /\ live h b /\ live h res /\ live h tmp /\
+		      disjoint res a /\ disjoint res b /\ disjoint res tmp))
+    (ensures  (fun h0 _ h1 -> preserves_live h0 h1))
+
+let rec karatsuba_ #aLen aaLen a b tmp res =
+    let tmpLen = mul #SIZE (size 4) aaLen in
+    let resLen = add #SIZE aaLen aaLen in
+    let aaLen2 = add #SIZE aaLen aaLen in
+    let aaLen0 = aaLen /. (size 2) in
+    assume (v aaLen = v aaLen0 + v aaLen0);    
+    fill resLen res (u64 0);
+    
+    if (aaLen <. size 9) then begin
+         bn_mul #aLen #aLen aaLen a aaLen b res end
+    else begin
+         let a0 = Buffer.sub #uint64 #aLen #(v aaLen0) a (size 0) aaLen0 in
+         let a1 = Buffer.sub #uint64 #aLen #(v aaLen0) a aaLen0 aaLen0 in
+         let b0 = Buffer.sub #uint64 #aLen #(v aaLen0) b (size 0) aaLen0 in
+         let b1 = Buffer.sub #uint64 #aLen #(v aaLen0) b aaLen0 aaLen0 in
+
+         let c0 = Buffer.sub #uint64 #(v resLen) #(v aaLen) res (size 0) aaLen in
+         let tmp0 = Buffer.sub #uint64 #(v tmpLen) #(v aaLen2) tmp (size 0) aaLen2 in
+         karatsuba_ #(v aaLen0) aaLen0 a0 b0 tmp0 c0; // c0 = a0 * b0
+
+         let c1 = Buffer.sub #uint64 #(v resLen) #(v aaLen) res aaLen aaLen in
+         let tmp1 = Buffer.sub #uint64 #(v tmpLen) #(v aaLen2) tmp aaLen aaLen2 in
+         karatsuba_ #(v aaLen0) aaLen0 a1 b1 tmp1 c1; // c1 = a1 * b1
+         
+         let a2 = Buffer.sub #uint64 #(v tmpLen) #(v aaLen0) tmp (size 0) aaLen0 in
+         let b2 = Buffer.sub #uint64 #(v tmpLen) #(v aaLen0) tmp aaLen0 aaLen0 in
+         let c2 = Buffer.sub #uint64 #(v tmpLen) #(v aaLen) tmp aaLen aaLen in
+         let tmp0 = Buffer.sub #uint64 #(v tmpLen) #(v aaLen2) tmp aaLen2 aaLen2 in
+	 
+         abs #(v aaLen0) aaLen0 a0 a1 a2; // a2 = |a0 - a1|
+         abs #(v aaLen0) aaLen0 b0 b1 b2; // b2 = |b0 - b1|
+         karatsuba_ #(v aaLen0) aaLen0 a2 b2 tmp0 c2; // c2 = a2 * b2
+
+	 let tmp1Len = add #SIZE aaLen (size 1) in
+         let tmp1 = Buffer.sub #uint64 #(v tmpLen) #(v tmp1Len) tmp aaLen2 tmp1Len in
+         add_sign #(v aaLen0) #(v aaLen) #(v tmp1Len) aaLen0 aaLen tmp1Len c0 c1 c2 a0 a1 a2 b0 b1 b2 tmp1; //tmp1 = (c0 + c1) +/- c2
+
+         //res = [c0; c1]
+         //tmp = [a2; b2; c2; tmp1; _]
+         let res1Len = add #SIZE aaLen0 aaLen in
+         let res1 = Buffer.sub #uint64 #(v resLen) #(v res1Len) res aaLen0 res1Len in
+         bn_add res1Len res1 tmp1Len tmp1 res1
+     end
+      
+    
+val karatsuba:
+    #aLen:size_nat ->
+    iLen:size_t{8 * v iLen < max_size_t} ->
+    aaLen:size_t{v aaLen == aLen /\ aLen + aLen < max_size_t /\ aLen <= v iLen} ->
+    a:lbignum aLen -> b:lbignum aLen ->
+    res:lbignum (aLen + aLen) -> Stack unit
+    (requires (fun h -> live h a /\ live h b /\ live h res /\ disjoint res a /\ disjoint res b))
+    (ensures  (fun h0 _ h1 -> preserves_live h0 h1 /\ modifies1 res h0 h1))
+    
+let karatsuba #aLen iLen aaLen a b res =
+    let tmpLen = mul #SIZE (size 4) iLen in
+    let stLen = add #SIZE tmpLen tmpLen in
+    let aaLen2 = add #SIZE aaLen aaLen in
+    
+    alloc #uint64 #unit #(v stLen) stLen (u64 0) [BufItem a; BufItem b] [BufItem res]
+    (fun h0 _ h1 -> True)
+    (fun st ->
+       let tmp = Buffer.sub #uint64 #(v stLen) #(v tmpLen) st (size 0) tmpLen in
+       let a_ = Buffer.sub #uint64 #(v stLen) #(v iLen) st tmpLen iLen in
+       let b_ = Buffer.sub #uint64 #(v stLen) #(v iLen) st (add #SIZE tmpLen iLen) iLen in
+       let res_ = Buffer.sub #uint64 #(v stLen) #(v iLen + v iLen) st (add #SIZE iLen (add #SIZE tmpLen iLen)) (add #SIZE iLen iLen) in
+       
+       let a_' = Buffer.sub #uint64 #(v iLen) #(aLen) a_ (size 0) aaLen in
+       let b_' = Buffer.sub #uint64 #(v iLen) #(aLen) b_ (size 0) aaLen in
+       
+       copy aaLen a a_';
+       copy aaLen b b_';
+       
+       karatsuba_ #(v iLen) iLen a_ b_ tmp res_;
+       
+       let res_' = Buffer.sub #uint64 #(v iLen + v iLen) #(aLen + aLen) res_ (size 0) aaLen2 in
+       copy aaLen2 res_' res;
+       admit()
+    )
